certicoq/theories/L4_deBruijn/L4_2_to_L5.v
@@ -318,7 +318,7 @@ Require Import Common.certiClasses.
 Local Instances are cleared at the end of a section.
 A more specific instance
 is redeclared in L4.instances using "Existing Instance" *)
-Local Instance L4aEval : BigStepOpSem NTerm := eval.
+Local Instance L4_2Eval : BigStepOpSem NTerm := eval.
 
 
 (** will be used in [eval_reduces_fvars] and cps_cvt_corr *)
